@@ -24,10 +24,10 @@ theorem release_br_ffffffffffffffb8 : KA.«release» + 0xffffffffffffffb8#64 = K
 theorem release_br_ffffffffffffff12 : KA.«release» + 0xffffffffffffff12#64 = KA.«holding» := by decide
 
 set_option maxHeartbeats 4000000 in
-theorem release_proof (HO : HOLDING) (PO : POPOFF) : RELEASE := ⟨
-  fun {hlc GF} _ _ cpu k γ s R _ hsie hnoff hK reen hreen hon => by
-  unfold wp_release_body
-  iintro ⟨Hk, Hpc, #Hlk, Hlocked, HR, Harm, HΦ⟩
+theorem release_hook_proof (HO : HOLDING) (PO : POPOFF) : RELEASE_HOOK := ⟨
+  fun {hlc GF} _ _ cpu k γ s R Rin _ hsie hnoff hK reen hreen hon => by
+  unfold wp_release_hook_body
+  iintro ⟨Hk, Hpc, #Hlk, Hlocked, HR, Hhook, Harm, HΦ⟩
   icases kctx_kernelText _ _ $$ Hk with ⟨#Htext, Hk⟩
   icases kctx_wf _ _ $$ Hk with ⟨%hwf, Hk⟩
   simp only [releaseAddr]
@@ -83,8 +83,8 @@ theorem release_proof (HO : HOLDING) (PO : POPOFF) : RELEASE := ⟨
   k_step (wp_s_fence_rw_w cpu _ (KA.«release» + 0x16#64) false 0#5 0#5) from (text_instr _ _ _ _ rfl rfl) Htext $$ [- $Hk $Hpc]
   iintro Hk Hpc
   -- sw zero,0(s1): the lock is free
-  k_step (wp_s_sw_zero_release cpu _ ?hs (KA.«release» + 0x1a#64) false 0#12 9#5 γ (k.regs 10#5) s R ?haddr) from (text_instr _ _ _ _ rfl rfl) Htext
-    $$ [- $Hk $Hpc $Hlp $Hheld $HR]
+  k_step (wp_s_sw_zero_release_hook cpu _ ?hs (KA.«release» + 0x1a#64) false 0#12 9#5 γ (k.regs 10#5) s R Rin ?haddr) from (text_instr _ _ _ _ rfl rfl) Htext
+    $$ [- $Hk $Hpc $Hlp $Hheld $HR $Hhook]
   case haddr => k_norm [h29]
   iintro Hk Hpc %hmem
   -- jal pop_off
